examples/riscv/mod2/mod2_symb_execScript.sml
@@ -27,53 +27,30 @@ Proof
    [bir_mod2_prog_def, mod2_prog_vars_def]
 QED
 
-(* ----------------------- *)
-(* Symbolic analysis setup *)
-(* ----------------------- *)
-
-val bprog_def = bir_mod2_prog_def;
-val init_addr_def = mod2_init_addr_def;
-val end_addr_def = mod2_end_addr_def;
-val bspec_pre_def = bspec_mod2_pre_def;
-val bprog_birenvtyl_def = mod2_birenvtyl_def;
-
-val bprog_tm = (snd o dest_eq o concl) bprog_def;
-val init_addr_tm = (snd o dest_eq o concl) init_addr_def;
-val end_addr_tm = (snd o dest_eq o concl) end_addr_def;
-val birs_state_init_lbl_tm = (snd o dest_eq o concl o EVAL)
- ``bir_block_pc (BL_Address (Imm64 ^init_addr_tm))``;
-val birs_state_end_lbls_tm = [(snd o dest_eq o concl o EVAL)
- ``bir_block_pc (BL_Address (Imm64 ^end_addr_tm))``];
-val bspec_pre_tm = (lhs o snd o strip_forall o concl) bspec_pre_def;
-val bprog_envtyl_tm = (fst o dest_eq o concl) bprog_birenvtyl_def;
-
-(* --------------------- *)
-(* Symbolic precondition *)
-(* --------------------- *)
-
-Theorem mod2_bsysprecond_thm =
- (computeLib.RESTR_EVAL_CONV [``birs_eval_exp``] THENC birs_stepLib.birs_eval_exp_CONV)
- ``mk_bsysprecond ^bspec_pre_tm ^bprog_envtyl_tm``;
-
-val birs_pcond_tm = (snd o dest_eq o concl) mod2_bsysprecond_thm;
-
 (* --------------------------- *)
 (* Symbolic analysis execution *)
 (* --------------------------- *)
 
 val timer = bir_miscLib.timer_start 0;
 
-val result = bir_symb_analysis bprog_tm
- birs_state_init_lbl_tm birs_state_end_lbls_tm
- bprog_envtyl_tm birs_pcond_tm;
+val (bsysprecond_thm, symb_analysis_thm) =
+ bir_symb_analysis_thms
+  bir_mod2_prog_def
+  mod2_init_addr_def mod2_end_addr_def
+  bspec_mod2_pre_def mod2_birenvtyl_def;
 
 val _ = bir_miscLib.timer_stop
  (fn delta_s => print ("\n======\n > bir_symb_analysis took " ^ delta_s ^ "\n"))
  timer;
 
 val _ = show_tags := true;
-val _ = Portable.pprint Tag.pp_tag (tag result);
 
-Theorem mod2_symb_analysis_thm = result
+val _ = Portable.pprint Tag.pp_tag (tag bsysprecond_thm);
+
+Theorem mod2_bsysprecond_thm = bsysprecond_thm
+
+val _ = Portable.pprint Tag.pp_tag (tag symb_analysis_thm);
+
+Theorem mod2_symb_analysis_thm = symb_analysis_thm
 
 val _ = export_theory ();
